#### Exercice a.
$$n = \frac{c}{v_{\varphi}} = \frac{c}{\omega}k \Leftrightarrow k = n \frac{2\pi}{Tc}$$
or : $Tc = \lambda_{0}$ et $k_{0}= \frac{2\pi}{Tc}$
$$\boxed{k =  nk_{0} \Leftrightarrow \lambda = \frac{\lambda_{0}}{n}}$$


#### Exercice b.
$$\varphi_{1}(x_{f}) = \varphi_{1}(x_{i}) + 2\pi\left( \frac{x_{f}-x_{i}-e}{\lambda_{0}} + \frac{1}{\lambda }e \right)$$
$$ =  \varphi_{1}(x_{i}) + 2\pi\left( \frac{x_{f}-x_{i}-e}{\lambda_{0}} + n\frac{1}{\lambda_{0} }e \right)$$
$$ =   \varphi_{1}(x_{i}) + \frac{2\pi}{\lambda_{0}}\left( x_{f}-x_{i}+(x-1)e \right)$$
Puis
$$\varphi_{2}(x_{f}) = \varphi_{2}(x_{i}) + 2\pi\left( \frac{x_{f}-x_{i}-e-\Delta e}{\lambda_{0}} + \frac{1}{\lambda }(e+\Delta e) \right)$$
$$\varphi_{2}(x_{f}) = \varphi_{2}(x_{i}) + \frac{2\pi}{\lambda_{0}}\left( x_{f}-x_{i} + (e+\Delta e)(n-1) \right)$$
Ainsi,
$$\boxed{\varphi_{2}(x_{f})- \varphi_{1}(x_{f}) = \frac{2\pi}{\lambda_{0}}(n -1)\Delta e}$$



$$\varphi = $$