# Exercice 3
## a.
BF : $u_{s} = R \times 0 = 0$
HF : $u_{s} = 0$

## b.
PDT
$$\underline{H} = \frac{\frac{1}{3}}{1+j \frac{1}{3}\left( x-\frac{1}{x} \right)}$$
$Q = \frac{1}{3}$
$$G = \frac{\frac{1}{3}}{\sqrt{ 1 + Q^{2}\left( x-\frac{1}{x} \right)^{2} }}\Rightarrow G_{\max} = G(x = 1) = \frac{1}{3}$$
$$G(\omega_{c}) = \frac{G_{\max}}{\sqrt{ 2 }} = \frac{1}{3\sqrt{ 2 }}$$
Alors, 
$$Q\left( x_{c}-\frac{1}{x_{c}} \right) = \pm1$$
Donc, 
$$x_{c}^{2} \pm \frac{1}{Q}x_{c} -1 = 0$$
Ainsi, 
$$x_{c} = \pm \frac{1}{2Q} \pm \frac{1}{2}\sqrt{ \frac{1}{Q^{2}} + 4}$$
Donc, 
$$x_{c} = \frac{\sqrt{ 13 }\pm3}{2}$$
