$$\sum_{n = 1}^{+ \infty} \frac{(-1)^{n}}{n!}(x\ln(x))^{n} - \frac{1}{x^{x}}$$
$$-\int _{0}^{1} (-x)^{x} \, dx $$
$$\sum_{}$$
$x = e^{ -t }$
$$J = \int_{0}^{1}\sum_{n = 1}^{+ \infty} f_{n} \, dx $$
$f_{n}$ est cont sur $[0, 1]$ et $\sum f_{n}$ CVS alors, 
$$J= \sum_{n = 1}^{+ \infty} \int_{0}^{1} f_{n}(t) \, dt = \sum_{n = 1}^{+\infty} J_{n} $$
$$J_{n} = \frac{(-1)^{n}}{n!}\int_{0}^{1} (x\ln(x))^{n} \, dx  = -\frac{(-1)^{n}}{n!} \int _{+ \infty}^{0} (-te^{ -t })^{n} e^{ -t } \, dt = \frac{1}{n!}\int _{0}^{+  \infty} t^{n}e^{ -(n+1)t } \, dt $$
$$x = e^{ -t }$$
$$dx = -e^{ -t } dt$$
$$\frac{1}{n!(x+1)^{n+1}}\int _{0}^{+ \infty} x^{n} e^{ -x } \, dx $$
On pose : $x = (n+1)t$ $dt = \frac{dx}{n+1}$

$$J_{n} = \frac{1}{(x+1)^{n+1}}$$


$$2^{-20}\leq 10^{-6}$$
$$(-1)^{n-1} \times e^{ -x\ln(n) }$$

$$(-1)^{n} \frac{\ln(n)}{n^{x}}$$
APDCR $n_{0}$ $\uparrow$ décroit donc d'après libeniz $\sum$ CV et puis, 
$$\left|\left| \sum_{k = 1}^{n}f'_{k}-\sum_{k = n+1}^{+ \infty}f'_{k} \right|\right| _{\infty, [a, + \infty[} = \left| R_{n}\right| \leq \frac{\ln(n+1)}{(n+1)^{x}}\leq \left|\left| x\mapsto \frac{\ln(n+1)}{(n+1)^{x}} \right|\right|_{\infty, [a, + \infty[} = \frac{\ln(n+1)}{(n+1)^{a}} \underset{n \to +\infty}{\longrightarrow} 0$$

$$T(x)-Z(x) = \sum_{n = 1}^{+ \infty} \frac{(-1)^{n+1}-1}{n^{x}} = -2\sum_{\underset{n \text{ pairs}}{n = 1}}^{+ \infty} \frac{1}{n^{x}}= -2 \sum_{k = 1}^{+ \infty} \frac{1}{(2k)^{x}} = -2^{1-x} Z(x)$$
$$ \sum_{\underset{n \text{ impairs}}{n = 1}}^{+ \infty} \frac{2}{n^{x}} -2Z(x) = \sum_{k = 0}^{+ \infty} \frac{2}{(2k+1)^{x}}-2$$

$$T(1+h) =(1-2^{-h}) Z(1+h) = \frac{\pi^{2}}{12}$$
$$2^{-h} = e^{ -h \ln(2)} = 1+h\ln(2)-\frac{h^{2}}{2}\ln^{2}(2)$$
	 