$$0= qE- fv \Rightarrow v = \frac{qE}{f}$$

$$\vec{j} = \rho \vec{v} = \frac{n q^{2}}{f}\vec{E} = \gamma \vec{E}$$
$\gamma$ le coefficient de conductivité
$$\frac{f}{nq}\vec{j} = q\vec{E} + q\vec{v} \wedge \vec{e}_{z} = q\vec{E} + \frac{1}{n} \vec{j} \wedge \vec{B}$$
Alors, 
$$\frac{nq^{2}}{f}\vec{E} + \frac{q^{2}n}{fnq} \vec{j} \wedge \vec{B}-\vec{j}= \gamma \vec{E} + \mathcal{R}\gamma \vec{j} \wedge \vec{B} - \vec{j}=0$$


$$\vec{E} + \mathcal{R} \vec{j} \wedge \vec{B}-\frac{1}{\gamma}\vec{j} = \overrightarrow{0}$$
$$div(\vec{j})=0$$
$$\overrightarrow{rot}(\vec{j}\wedge \vec{B}) = \frac{1}{\gamma \mathcal{R}} \overrightarrow{rot}(\vec{j})$$

$$div(\vec{E}) = \frac{nq}{\varepsilon_{0}} = -\mathcal{R} div(\vec{j} \wedge \vec{B})$$

$$0 = div(\vec{j}) = - \frac{\partial qn}{\partial t} =- \frac{\partial \varepsilon_{0} div(\vec{E})}{\partial t} = div\left( -\varepsilon_{0}\frac{\partial E}{\partial t}  \right)$$

$$qn = \text{cte}$$

$$\overrightarrow{rot}(\vec{j} \wedge \vec{B}) = \vec{j} div(\vec{B}) - (\vec{j} . \overrightarrow{grad}) \vec{B} - \vec{B} div(\vec{j}) + \vec{B} . \overrightarrow{grad}(\vec{j}) = 0$$

$$\vec{E} = \frac{1}{\gamma}\vec{j} - \mathcal{R} \vec{j} \wedge \vec{B}$$

$$u = \int_{Q}^{P} \vec{E}.d\vec{l} = \int_{Q}^{P} \vec{E}.\vec{e}_{x} dx+ \int_{Q}^{P} E_{y}dy = lE_{y}$$

$$R = \frac{lE_{y}}{i}$$
Soit $d\vec{S}$ orienté // à $\vec{j}$ : 
$$$$