#### Exercice a.
$$ \frac{\partial \underline{\vec{v}}}{\partial t}  = -\frac{q}{m}\underline{\vec{E}} = -\frac{q}{m}\overrightarrow{\underline{E}}_{0} e^{ i(\omega t - \vec{k}.\vec{r}) }$$

Alors, la vitesse d'un éléctron est : 
$$\underline{\vec{v}} = i\frac{q}{\omega m} \underline{\overrightarrow{E_{0}}} e^{ i(\omega t-\vec{k}.\vec{r}) } = i \frac{q}{\omega m} \underline{\overrightarrow{E}}$$
celle de $N$ électrons est : $N\vec{v}$
Alors, 
$$\vec{j} = Nqn_{0} \vec{v} = \frac{i n_{0}q}{\omega m} \vec{E}$$
en posant
$$\underline{\gamma} = \frac{i\rho q}{\omega m}$$
$$\vec{j}= \underline{\gamma} \vec{E}$$
