
#### DÃ©monstration de l'expression de $\vec{a}(M / \mathcal{R})$
$$\vec{a}(M / \mathcal{R}) = \frac{d\vec{v}(M / \mathcal{R})}{dt}_{\mathcal{R}}$$
$$\frac{d\vec{v}(M / \mathcal{R})}{dt}_{\mathcal{R}} = \frac{d\vec{v}(M / \mathcal{R}')}{dt}_{\mathcal{R}} + \frac{d^{2}OO'}{dt^{2}}_{\mathcal{R}} + \frac{d\omega(\mathcal{R}' / \mathcal{R})}{dt}_{\mathcal{R}} \wedge \vec{r'}$$
$$+ \omega(\mathcal{R}'/\mathcal{R})\wedge \frac{d\vec{r'}}{dt}_{\mathcal{R}}$$
Comme : 
$$\frac{d\vec{v}(M / \mathcal{R}')}{dt}_{\mathcal{R}} = \frac{d\vec{v}(M / \mathcal{R}')}{dt}_{\mathcal{R}'} + \omega(\mathcal{R}' / \mathcal{R}) \wedge \vec{v}(M / \mathcal{R}')$$
et 
$$\frac{dr'}{dt}_{\mathcal{R}} = \frac{dr'}{dt}_{\mathcal{R}'} + \omega(\mathcal{R}' / \mathcal{R}) \wedge r'_{}$$
Donc, 

$$\vec{a}(\mathcal{M} / \mathcal{R}) =\vec{a}(M / \mathcal{R}') + \vec{a}(O' / \mathcal{R}) + \frac{d\omega}{dt}_{\mathcal{R}} \wedge \overrightarrow{r'} + \omega \wedge (\omega \wedge \overrightarrow{r'}) + 2 \omega \wedge \overrightarrow{v'}$$

