#### 1.
$$\frac{\partial T}{\partial t} = \frac{T^{n+1}-T^{n}}{\Delta t} \text{ et } \frac{\partial T}{\partial x}  = \frac{T_{j-1}-T_{j}}{\Delta x} \text{ alors } \frac{\partial^{2} T}{\partial x^{2}} = \frac{T^{n}_{j-1}-2T ^{n}_{j}+T ^{n}_{j+1}}{(\Delta x)^{2}} $$
Donc, 

#### 2.
$$\frac{\partial T^{*}}{\partial t^{*}} = \frac{\partial^{2}T^{*}}{\partial (x^{*})^{2}}  $$
	
#### 3.
$$D_{th} = \frac{\lambda}{\mu c_{v}} $$
$$\frac{\phi}{S} = -\lambda \frac{\Delta T}{\Delta x}$$
$$\lambda = -\frac{S\Delta x}{\phi \Delta T}$$
$$S = 2\times 10^{-4}$$

$$d = 10r$$