### Exercice 2
#### 1.
$$\underline{\overrightarrow E} = \underline{\overrightarrow{E_{0}}}e^{ i(\omega t - \vec{k}.\vec{r}) }$$
Comme l'onde se propage selon $\vec{e}_{x}$ : $\vec{k} = \vec{e}_{x}$
$$\vec{E}.\vec{e}_{y} = E_{0} \cos\left( \frac{\pi}{3} \right) = \frac{E_{0}}{2}$$
$$\vec{E}.\vec{e}_{z} = E_{0}\cos\left( \frac{\pi}{6} \right) = \frac{E_{0}\sqrt{3}}{2}$$
De plus : 
$$\vec{E} = E_{0} \cos(\omega t-kx + \varphi)\begin{pmatrix}
0 \\
\frac{1}{2} \\
\frac{\sqrt{3}}{2}
\end{pmatrix}$$

#### 2.
$$\vec{k} = k\left( \cos\left( \frac{\pi}{4} \right)\vec{e}_{x} +\cos\left( \frac{\pi}{4} \right) \vec{e}_{z}\right)= k \frac{\sqrt{2}}{2} (\vec{e}_{x} + \vec{e}_{z})$$

Ainsi,
$$\vec{E} = E_{0} \cos\left( \omega t - k \frac{\sqrt{2}}{2}(x+y) + \varphi \right)\vec{e}_{y}$$

### Exercice 4
#### 1.
##### a.
$$\vec{\nabla} = \begin{pmatrix}
\frac{\partial }{\partial x}  \\
\frac{\partial }{\partial y}  \\
\frac{\partial }{\partial z} 
\end{pmatrix}$$
	