## Question 1
#### a.
On a : $\forall k \in \mathbb{N}, \frac{X_{k}+1}{2} \sim B(p)$ ou $p = \frac{1}{2}$ donc :
$$\forall n \in \mathbb{N}, \frac{S_{n}}{2}+ \frac{n}{2} \sim B(n, p)$$
alors, 
$$T_{2n} = \frac{S_{2n}}{2} + n \sim B(2n, p)$$

$$\forall n \in \mathbb{N}, \mathbb{P}\left( S_{2n} = 0 \right) = \mathbb{P}(T_{2n} = n) = \binom{2n}{n} 4^{-n} $$

#### b.
$$\mathbb{P}(S_{2n} = 0) = \binom{2n}{n} 4^{-n} = \frac{(2n)!}{(n!)^{2} 4^{n}}$$
$$\sim_{+ \infty} \frac{2\sqrt{\pi n}\left( \frac{2n}{e} \right)^{2n}}{2\pi n \left( \frac{n}{e} \right)^{2n} 4^{n}} = \frac{1}{\sqrt{\pi n}} \underset{n \to +\infty}{\longrightarrow} 0$$
$$\mathbb{P}(S_{2n+1} = 0) = 0$$
Ainsi, 
$$\mathbb{P}(S_{n} = 0) \underset{n \to +\infty}{\longrightarrow} 0$$

$$\mathbb{P}(S_{n} \leq 0) = 1- \mathbb{P}(S_{n} > 0) = 1- \sum_{k = 1}^{n}\mathbb{P}(S_{n} = k)  $$
$$\mathbb{P}\left( T_{n} = \frac{k+n}{2} \right) = \binom{n}{\frac{k+n}{2}} 2^{-n}$$

## Question 2
#### a.
$$\frac{1}{2\pi} \int_{-\pi}^{\pi} \mathbb{E}(e^{ itX }) e^{ -itk } \, dt = \frac{1}{2\pi}  \sum_{j = -n}^{n}\mathbb{P}(X = j)\int_{-\pi}^{\pi}e^{ it(j-k) } \, dt$$
$$= \frac{1}{\pi} \sum_{\underset{j \neq k}{j = -n}}^{n} \frac{\mathbb{P}(X = j)}{j-k}\sin(\pi(j-k)) + \frac{1}{2\pi} \mathbb{P}(X = k) \int_{-\pi}^{\pi}  \, dt$$
$$= \mathbb{P}(X = k)$$

#### b.
$$\mathbb{E}(e^{ itS_{n} }) = \prod_{k = 1}^{n} \mathbb{E}(e^{ itX_{k} }) = \cos(t)^{n}$$
$$\mathbb{E}(e^{ itX_{k} }) = \mathbb{P}(X= -1) e^{ -it } + \mathbb{P}(X = 1 ) e^{ it } = \frac{e^{ it }+e^{ -it }}{2} = \cos(t)$$

## Question 3
#### a.
$$ \mathbb{P}\left( 0 < S_{b} \leq b\sqrt{n} \right) = \sum_{k = 1}^{\left\lfloor b\sqrt{n}
\right\rfloor } P(X = k) = \dots
$$

#### b.
$$\mathbb{P}\left( 0 < \frac{S_{n}}{\sqrt{n}} \leq b\right) = \frac{1}{2\pi} \int_{-\pi}^{\pi} (\cos(t))^{n} \sum_{k = 1}^{\left\lfloor b\sqrt{n} \right\rfloor} e^{ -itk } \, dx $$
$$\mathbb{P}(\dots) = \dots$$

#### c.

## Question 4
#### a.
$$f_{n}(x) \sim \left( \cos\left( \frac{x}{\sqrt{n}} \right) \right)^{n} \frac{1-e^{ -ixb }}{\left( \frac{ix}{\sqrt{n}} \right)\sqrt{n}} \sim \cos\left( \frac{x}{\sqrt{n}} \right)^{n} \frac{1-e^{ -ixb }}{ix}$$
$$\cos\left( \frac{x}{\sqrt{n}} \right)^{n} = \left( 1-\frac{x^{2}}{2n} + o\left( \frac{1}{n} \right) \right)^{n} = e^{ n\ln\left( 1-\frac{x^{2}}{2n} + o\left( \frac{1}{n} \right) \right) }$$
$$= e^{ -n\left( \frac{x^{2}}{2n} - o\left( \frac{1}{n} \right) \right)  } = e^{-\frac{x^{2}}{2} + o(1) } \underset{n \to +\infty}{\longrightarrow} e^{ -\frac{x^{2}}{2} }$$
Ainsi, 
$$f_{n}(x) \underset{n \to +\infty}{\longrightarrow}  e^{ -\frac{x^{2}}{2} } \frac{1-e^{ -ixb }}{ix}$$
