# Niveau 1 (CCP)
## Exercice 1
#### 1.
Par le TMC : 
$$\frac{d ml (\vec{e}_{l} \wedge \vec{v})}{dt} = lm(\vec{e}_{l}\wedge \vec{g}) + \overrightarrow{0} - 6l\pi \eta r ( \vec{e}_{l}\wedge \vec{v}) $$
Alors,
$$ \dot{\theta} (\vec{e}_{\theta} \wedge \vec{v}) +  \left( \vec{e}_{l} \wedge \frac{d\vec{v}}{dt} \right) =-g\sin(\theta) \vec{e}_{z} - \frac{6\pi \eta r}{m} \vec{e}_{z} $$

$$\vec{l} = l \vec{e}_{l} \text{ alors } \vec{v} = l\dot{\theta} \vec{e}_{l} \text{ et } \vec{a} = l(\ddot{\theta} \vec{e}_{l} - \dot{\theta}^{2}\vec{e}_{\theta} )$$
Alors, en projettant sur $\vec{e}_{z}$ : 
$$-l\dot{\theta}^{2} \vec{e}_{z} - l\dot{\theta}^{2}\vec{e}_{z} = -2l\dot{\theta}^{2} = -g \sin(\theta) - \frac{6\pi \eta r}{m} $$
Ainsi, 
$$\boxed{\dot{\theta}^{2} - \frac{g}{2l}\sin(\theta) = \frac{6\pi \eta r}{m}}$$
