$$e^{ x } \underset{x \to 0}{=} 1+x+\frac{x^{2}}{2} + o(x^{2})$$
$$\frac{1}{1+x^{2}} = 1-x^{2} + o(x^{2})$$
Alors, 
$$\int \frac{1}{1+x^{2}} \, dx = Arctan(x) = x-\frac{1}{3}x^{3} + o(x^{3})$$

$$e^{ x }\arctan(x) \underset{x \to 0}{=}  x+x^{2} + \frac{x^{3}}{6} + o(x^{3})$$
____
$$\sin(2x) \underset{x \to 0}{=} 2x-4\frac{x^{3}}{3} + o(x^{3})$$
$$\frac{1}{\sqrt{ 1+x }} = (1+x)^{-\frac{1}{2}} = 1-\frac{x}{2} + \frac{x^{2}}{4} + o(x^{2}) $$
Alors, 
$$\frac{\sin(2x)}{\sqrt{ 1+x }} \underset{x \to 0}{=} 2x-x^{2}-\frac{5x^{3}}{6} + o(x^{3})$$

# Exercice 1
## (a). 
$$\sum_{k = 0}^{n}e^{ ikx } + \sum_{k = 0}^{n}e^{ -ikx} = \frac{1-e^{ ix(n + 1) }}{1-e^{ ix }} + \frac{1-e^{ -ix(n + 1) }}{1-e^{ -ix }}$$
$$=  \frac{(e^{ ix })^{-n} - (e^{ ix })^{n+1}}{1-e^{ ix }} = \frac{e^{ \frac{ix}{2} }\left( e^{ -i\left( n + \frac{1}{2} \right)x }- e^{ i\left( n+ \frac{1}{2} \right)x } \right)}{e^{ i \frac{x}{2} }\left( e^{ - \frac{ix}{2} } + e^{ \frac{ix}{2} } \right)} $$
Ainsi, 
$$\sum_{k = -n}^{n} e^{ ikx } = \frac{\sin\left( \left( n+\frac{1}{2} \right)x \right)}{\sin\left( \frac{x}{2} \right)}$$

### (b).
$$\sum_{n = -\infty}^{+ \infty} r^{\left| n\right|}e^{ inx } = \sum_{n = 0}^{+ \infty}r^{n} e^{ inx } + \sum_{n = 1}^{+ \infty} r^{-n}e^{ -inx } $$
$$=  \sum_{n= 0}^{+ \infty} (re^{ ix })^{n}+ \sum_{n = 0}^{+ \infty}(re^{ ix })^{-n}-1$$
Alors, 
$$\sum_{n = 0}^{+ \infty}(r e^{ ix })^{n} = \lim_{ m \to \infty } \frac{1-r^{m}e^{ ixm +1 }}{1-re^{ ix }} $$
et
$$\sum_{n = 0}^{+ \infty}\left( \frac{1}{r e^{ ix }} \right)^{n} = \lim_{ m \to \infty } \frac{1-r^{-m}e^{ -ixm -1 }}{1-\frac{e^{ -ix }}{r}}$$
$$ = \lim_{ m \to \infty } - r e^{ ix }\frac{1-r^{-m}e^{ -ixm-1 }}{1-re^{ ix }} $$
Alors, 
$$\sum_{n = - \infty}^{+ \infty} r^{\left| n\right|}e^{ inx } = \lim_{ m \to \infty }  \frac{}{}$$
etc...

### (c).
$$\sum_{k =0}^{n} \sum_{j = 0}^{k}e^{ ixj } = \sum_{j = 0}^{n}\sum_{k=j}^{n} e^{ ixj } = \sum_{j = 0}^{n} (n-j+1)e^{ ixj }=D_{n}(x)$$

# Exercice 2
### (a). 
On fait une première IPP : 
$$\begin{cases}
u = \cos ^{n}(t) \\
du = -n\sin(t)\cos ^{n-1}(t)dt
\end{cases} \text{ et } \begin{cases}
v = \frac{1}{c}\sin(ct) \\
dv = \cos(ct)dt
\end{cases}$$

$$I_{n}(c) = \frac{1}{c}[\cos ^{n}(t)\sin(ct)]_{0}^{\frac{\pi}{2}} + \frac{n}{c}\int_{0}^{\frac{\pi}{2}} \sin(t)\sin(ct)\cos ^{n-1}(t)   \, dt $$
On fait une deuxième IPP : 
$$\begin{cases}
u =  -\frac{1}{c}\cos(ct)\\
du = \sin(ct)dt
\end{cases} \text{ et } \begin{cases}
v = \sin(t) \cos(t)^{n-1} \\
dv = (\cos ^{n}(t) - (n-1)\sin ^{2}(t)\cos ^{n-2}(t))dt
\end{cases}$$
$$\int _{0}^{\frac{\pi}{2}} \sin(t)\sin(ct)\cos ^{n-1}(t) \, dt $$
$$= \frac{n}{c}\left( \left[ (\sin(t))(\cos(t))^{n-1}-\frac{\cos(ct)}{c} \right]_{0}^{\frac{\pi}{2}}\right.$$
$$-\left.\int _{0}^{\frac{\pi}{2}} (\cos ^{n}(t) - (n-1)\sin ^{2}(t)\cos ^{n-2})\left( \frac{\cos(ct)}{c} \right) \, dt  \right)$$
$$= \frac{n}{c^{2}} \int _{0}^{\pi/2}((\cos ^{n}(t))\cos(ct)-(n-1) \sin ^{2}(t) \cos(ct)\cos ^{n-2}(t)) \, dt $$
$$= \frac{n}{c^{2}}\left( I_{n}(c) - (n-1)\int _{0}^{\pi/2} (\cos ^{n-2} t\cos(ct) - \cos ^{n} t\cos(ct)) \, dt  \right)$$
$$= \frac{n}{c^{2}}(I_{n}(c) -(n-1)(I_{n-2}(c)-I_{n}(c)))$$
Ainsi, 
$$c ^{2}I_{n} = nI_{n}-n(n-1)(I_{n-2}-I_{n})$$
Soit : 
$$(n^{2}-c^{2})I_{n}(c) =n(n-1)I_{n-2}(c)$$
### b.
Remplaçons $n$ par $2n$, 
En évaluant en $0$ on a l'exp finale

