### Exercice 7
#### a.
$$\left| \sin(x+iy)\right|^{2}  = \frac{1}{4} \left| e^{ i(x+iy) } - e^{ -i(x+iy) } \right|^{2} = \frac{1}{4}\left| (e^{ i(x+iy) }-e^{ -i(x+iy) })(e^{ -i(x+iy) }-e^{ i(x+iy) }) \right|$$

$$= \frac{1}{4} \left (e^{ ix }e^{ -y }-e^{ -ix }e^{ y }\right) \left( e^{ -ix }e^{ -y }-e^{ ix }e^{y } \right)$$
$$= \frac{1}{4}(e^{ -2y } - e^{ -2ix } - e^{ 2ix }+ e^{ 2y }) $$
$$= \frac{ch(2y) - \cos(2x)}{2}$$

$$\frac{\partial f}{\partial x}(x, y) = \sin(2x)$$
$$\frac{\partial f}{\partial y} (x, y) = sh(2y)$$
$sh$ s'anneleuuuuh pour $y = 0$ et $x \equiv \frac{\pi}{2}$