### Question 1
#### a.
$x\mapsto (1-x)^{-\frac{1}{2}}$ est développable en série entière usuelle
$$\forall x \in [0, 1[, \frac{1}{\sqrt{1-x}} = (1-x)^{-\frac{1}{2}} = \sum_{n =0}^{+ \infty} \frac{\underset{k=1}{\overset{n}{\prod}}\left( -\frac{1}{2}-(k-1) \right)}{n!} (-x)^{n} = \sum_{n=0}^{+ \infty} \frac{2^{-n}\underset{k=1}{\overset{n}{\prod}}\left( 1+2(k-1) \right)}{n!} x^{n}$$
$$=\sum_{n=0}^{+ \infty} \frac{2^{-n}}{n!} \left( \prod_{k = 1}^{n-1} (2k+1) \right) x^{n} = \sum_{ n= 0}^{+ \infty} \frac{2^{-n}}{n!} \frac{\underset{k=1}{\overset{n}{\prod}}(2k)(2k+1)}{\underset{k=1}{\overset{n}{\prod}}} x^{n} $$